src/Reflect.v
@@ -243,6 +243,29 @@ Ltac indexOf keyF x ls :=
       end
   end.
 
+Ltac map_tac T tac fs :=
+  let rec map_tac fs :=
+    match fs with
+      | nil => constr:(@nil T)
+      | ?f :: ?fs =>
+        let f := tac f in
+        let fs := map_tac fs in
+        constr:(f :: fs)
+      | ?fs ++ ?fs' =>
+        let fs := map_tac fs in
+        let fs' := map_tac fs' in
+        constr:(fs ++ fs')
+      | _ => 
+        let fs' := eval unfold fs in fs in 
+        match fs with
+          | fs' => fs
+          | _ => map_tac fs'
+        end
+    end
+  in
+  map_tac fs.
+  
+
 Goal forall a b c : Type, nil ++ (a :: nil) ++ nil ++ nil = nil.
   intros.
   match goal with
